LeanSAT/Data/PPA.lean
@@ -1,0 +1,664 @@
+import LeanSAT.Data.Cnf
+import LeanSAT.Data.ICnf
+import LeanSAT.AuxDefs
+import LeanSAT.Upstream.ToStd
+import Mathlib.Data.Nat.Basic
+
+open LeanSAT LeanSAT.Model Nat
+
+/-- A partial assignment of truth values to propositional variables.
+
+It is meant to be kept around persistently and used linearly.
+Assuming these restrictions are met,
+the structure provides a fast and allocation-free representation
+of partial assignments.
+It provides functions for unit propagation and tautology checking. -/
+structure PPA where
+  assignment : Array Int
+  /-- The generation counter is used to avoid clearing the assignment array.
+  Instead, we just bump the counter and interpret values in the array
+  below the counter as unassigned. -/
+  generation : { g : Nat // g > 0 }
+  /-- The maximum absolute value of any entry in `assignments`. -/
+  maxGen : Nat
+
+namespace PPA
+  open LitVar
+
+@[reducible] def size (τ : PPA) : Nat := τ.assignment.size
+
+  /-- The value of the given literal in the current assignment, if assigned.
+  Otherwise `none`. -/
+def litValue? (τ : PPA) (l : ILit) : Option Bool :=
+  match τ.assignment.get? ((toVar l).val - 1) with
+  | none => none
+  | some n =>
+    if τ.generation.val ≤ n.natAbs then
+      some <| xor (n < 0) (polarity l)
+    else
+      none
+
+  -- Cayden: Alternative definition that uses a let, not a match:
+  --let v := τ.assignment.getD ((toVar l).val - 1) 0
+  --if τ.generation ≤ v.natAbs then
+  --  some <| xor (v < 0) (polarity l)
+  --else none
+
+def varValue? (τ : PPA) (v : IVar) : Option Bool :=
+  τ.litValue? (mkPos v)
+
+-- Cayden TODO: There's a far more elegant proof here
+theorem litValue?_negate (τ : PPA) (l : ILit) :
+    τ.litValue? l = Option.map Bool.not (τ.litValue? (-l)) := by
+  unfold litValue?
+  match hlit : Array.get? τ.assignment ((toVar l).val - 1) with
+  | none => simp [hlit, -Array.get?_eq_getElem?]
+  | some n =>
+    simp [hlit, -Array.get?_eq_getElem?]
+    by_cases hτ : τ.generation.val ≤ Int.natAbs n
+    <;> cases polarity l <;> by_cases hn : (n < 0) <;> simp [hτ, hn]
+
+theorem litValue?_eq_varValue?_none {τ : PPA} {l : ILit} :
+    τ.litValue? l = none → τ.varValue? (toVar l) = none := by
+  simp only [litValue?, varValue?]
+  cases hlit : Array.get? τ.assignment ((toVar l).val - 1)
+  <;> simp [hlit, -Array.get?_eq_getElem?]
+
+theorem litValue?_eq_varValue?_some {τ : PPA} {l : ILit} {b : Bool} :
+    τ.litValue? l = some b → τ.varValue? (toVar l) = xor (!b) (polarity l) := by
+  simp only [litValue?, varValue?]
+  cases hlit : Array.get? τ.assignment ((toVar l).val - 1) with
+  | none => simp [hlit, -Array.get?_eq_getElem?]
+  | some n =>
+    simp [hlit, -Array.get?_eq_getElem?]
+    by_cases hτ : τ.generation.val ≤ Int.natAbs n
+    <;> cases polarity l <;> by_cases hn : (n < 0) <;> cases b <;> simp [hτ, hn]
+
+theorem lt_size_of_litValue?_eq_some {τ : PPA} {l : ILit} {b : Bool} :
+    τ.litValue? l = some b → ((toVar l).val - 1) < τ.size := by
+  sorry
+  done
+
+def toPropFun_fun (τ : PPA) : PropFun IVar → Fin τ.size → ℤ → PropFun IVar :=
+  fun acc idx a => acc ⊓
+    (if τ.generation ≤ a then .var ⟨idx.val + 1, succ_pos _⟩
+     else (.var ⟨idx.val + 1, succ_pos _⟩)ᶜ)
+
+def toPropFun (τ : PPA) : PropFun IVar :=
+  τ.assignment.foldlIdx (init := ⊤) (toPropFun_fun τ)
+
+theorem toPropFun_fun_comm (τ : PPA) :
+  ∀ (acc : PropFun IVar) (idx₁ idx₂ : Fin τ.size),
+    (toPropFun_fun τ) ((toPropFun_fun τ) acc idx₁ (τ.assignment.get idx₁)) idx₂ (τ.assignment.get idx₂) =
+    (toPropFun_fun τ) ((toPropFun_fun τ) acc idx₂ (τ.assignment.get idx₂)) idx₁ (τ.assignment.get idx₁) := by
+  intro acc i j
+  simp only [toPropFun_fun, Array.get_eq_getElem, ge_iff_le, le_inf_iff, inf_right_comm]
+
+instance : ToString PPA where
+  toString τ := String.intercalate " ∧ "
+    (τ.assignment.foldl (init := []) (f := fun acc a => s!"{a}" :: acc))
+
+end PPA
+
+-- ??
+--structure PPA.WF (ppa : PPA) where
+  -- hGen: 0 < generation
+  -- hMaxVal : ∀ x ∈ assignment, x.natAbs ≤ maxVal
+
+namespace PPA
+  open LitVar PropFun
+
+  /-- Initialize to an empty partial assignment,
+  supporting variables in the range `[1, maxVar]`.
+
+  The assignment will resize dynamically if it's used with
+  a variable above the initial `maxVar`. -/
+  def new (maxVar : Nat) : PPA where
+    assignment := Array.mkArray maxVar 0
+    generation := ⟨1, Nat.one_pos⟩
+    maxGen := 0
+
+  /-- Reset the assignment to an empty one. -/
+  def reset (τ : PPA) : PPA :=
+    { τ with generation := ⟨τ.maxGen + 1, Nat.succ_pos _⟩ }
+
+  /-- Clear all temporary assignments at the current generation. -/
+  def bump (τ : PPA) : PPA :=
+    { τ with generation := ⟨τ.generation + 1, Nat.succ_pos _⟩ }
+
+  /-- Set the given literal to `true` for the current generation
+  in the assignment. -/
+  def setLit (τ : PPA) (l : ILit) : PPA :=
+    let v : Int := if polarity l then τ.generation else -τ.generation
+    { τ with
+      assignment := τ.assignment.setF ((toVar l).val - 1) v 0
+      maxGen := Nat.max τ.maxGen τ.generation }
+
+  /-- Set the given literal to `true` for all generations until `gen`. -/
+  def setLitUntil (τ : PPA) (l : ILit) (gen : Nat) : PPA :=
+    let v : Int := if polarity l then gen else -gen
+    { τ with
+      assignment := τ.assignment.setF ((toVar l).val - 1) v 0
+      maxGen := Nat.max τ.maxGen gen }
+
+  /-- Check if the given clause is a tautology.
+  The current partial assignment is ignored,
+  and the assignment afterwards is unspecified. -/
+  def checkTauto (τ : PPA) (C : IClause) : PPA × Bool := Id.run do
+    let mut τ := τ.reset
+    for l in C do
+      if let some false := τ.litValue? l then
+        return (τ, true)
+      τ := τ.setLit l
+    return (τ, false)
+
+  /-- Set `l ↦ ⊥` for each `l ∈ C` and leave the rest of the assignment untouched.
+  If the current assignment contains literals appearing in `C`, they will be overwritten. -/
+  -- NB: might be easier to verify if we make this always bump p.generation; it's only used before UP anyway
+  -- left without bump but might result in harder theorem
+  def setNegatedClause (τ : PPA) (C : IClause) : PPA :=
+    C.foldl (init := τ) (fun τ l => τ.setLit (-l))
+
+  def setNegatedClauseUntil (τ : PPA) (C : IClause) (gen : Nat) : PPA :=
+    C.foldl (init := τ) (fun τ l => τ.setLitUntil (-l) gen)
+
+  /-! # Lemmas -/
+
+  theorem setLit_pos (τ : PPA) (l : ILit) : (τ.setLit l).litValue? l = some true := by
+    rw [litValue?, setLit]
+    cases polarity l
+    <;> simp [Array.getElem?_setF]
+    exact τ.generation.property
+
+  theorem setLit_neg (τ : PPA) {l l' : ILit} :
+      (toVar l) ≠ (toVar l') → (τ.setLit l).litValue? l' = τ.litValue? l' := by
+    intro hl
+    simp only [litValue?, setLit]
+    have : (toVar l).val - 1 ≠ (toVar l').val - 1 := by
+      rcases ILit.exists_succ_toVar l with ⟨n₁, hn₁⟩
+      rcases ILit.exists_succ_toVar l' with ⟨n₂, hn₂⟩
+      rw [hn₁, hn₂, Nat.add_sub_cancel, Nat.add_sub_cancel]
+      -- TODO: How to use ≠ instead of ¬( = )?
+      have := mt Subtype.ext hl
+      have : ↑(toVar l) ≠ (toVar l').val := this
+      simp [hn₁, hn₂] at this
+      exact this
+    cases polarity l
+    <;> simp [Array.getElem?_setF' _ _ _ this]
+
+  theorem setLit_varValue_pos (τ : PPA) {l : ILit} {v : IVar} :
+      v = (toVar l) → (τ.setLit l).varValue? v = some (polarity l) := by
+    intro hv
+    rw [varValue?]
+    have h_setLit := setLit_pos τ l
+    cases hpol : polarity l
+    · have : (mkPos v) = -l := by rw [hv]; ext <;> simp [hpol]
+      rw [this]
+      rw [litValue?_negate] at h_setLit
+      match hlit : litValue? (setLit τ l) (-l) with
+      | none => simp [hlit] at h_setLit
+      | some b =>
+        cases b with
+        | true => simp [hlit] at h_setLit
+        | false => rfl
+    · have : (mkPos v) = l := by rw [hv]; ext <;> simp [hpol]
+      rw [this]
+      exact h_setLit
+
+  theorem setLit_varValue_neg (τ : PPA) {l : ILit} {v : IVar} :
+      (toVar l) ≠ v → (τ.setLit l).varValue? v = τ.varValue? v := by
+    intro hv
+    -- TODO: Why all the instances?
+    rw [← @LawfulLitVar.toVar_mkPos ILit IVar LeanSAT.instLitVarILitIVar
+      LeanSAT.instLawfulLitVarILitIVarInstLitVarILitIVar v] at hv
+    exact setLit_neg τ hv
+
+  #check PropFun.entails
+
+  theorem satisfies_iff {τ : PPA} {σ : PropAssignment IVar} :
+      σ ⊨ τ.toPropFun ↔ ∀ v b, τ.varValue? v = some b → σ v = b := by
+    constructor
+    · intro hσ v b hv
+      rw [toPropFun] at hσ
+      have := Array.foldlIdx_of_comm τ.assignment (toPropFun_fun τ) ⊤ (toPropFun_fun_comm τ)
+      --have ⟨a, ha⟩ := ⊤.fold_of_mapsTo_of_comm
+      --rw [toPropFun] at hσ
+
+      --rw [satisfies_iff] at hσ
+      sorry
+      done
+    · sorry
+
+    /-
+    where
+  mp := fun h => by
+    intro x p? hFind
+    have ⟨φ, hφ⟩ := τ.fold_of_mapsTo_of_comm
+      (init := ⊤) (f := fun acc x v => acc ⊓ if v then PropTerm.var x else (PropTerm.var x)ᶜ)
+      hFind ?comm
+    case comm =>
+      intros
+      dsimp
+      ac_rfl
+    rw [toPropTerm, hφ] at h
+    aesop
+
+  mpr := fun h => by
+    apply HashMap.foldRecOn (hInit := satisfies_tr)
+    intro φ x p hφ hFind
+    rw [satisfies_conj]
+    refine ⟨hφ, ?_⟩
+    have := h _ _ hFind
+    split <;> simp [*]
+    -/
+
+  theorem satisfies_iff' {τ : PPA} {σ : PropAssignment IVar} :
+      σ ⊨ τ.toPropFun ↔ ∀ l b, τ.litValue? l = some b → σ (toVar l) = xor (!b) (polarity l) := by
+    constructor
+    · intro hσ l b hl
+      have := satisfies_iff.mp hσ (toVar l) (xor (!b) (polarity l))
+      cases b
+      · simp at this
+        simp
+        apply this
+        unfold varValue?
+        sorry
+      · sorry
+    · sorry
+    done
+
+  /-! # Unit propagation -/
+
+  -- Propagate Partial result
+  inductive PPR where
+    | satisfied
+    | multipleUnassignedLiterals
+
+  --
+  inductive PropagateResult where
+    | contradiction
+    | extended (l : ILit) (τ : PPA)
+    | satisfied
+    | multipleUnassignedLiterals
+
+  /-- A result of `propagateUnit` on inputs `τ` and `C`. -/
+  inductive PropagateResultDep (τ : PPA) (C : IClause) where
+    | contradiction (h : C.toPropFun ⊓ τ.toPropFun = ⊥)
+    | extended      (l : ILit)
+                    (τ' : PPA)
+                    (h₁ : C.toPropFun ⊓ τ.toPropFun = τ'.toPropFun)
+                    (h₂ : τ.litValue? l = none ∧ τ'.litValue? l = some true)
+    | satisfied                    -- The clause was satisfied
+    | multipleUnassignedLiterals   -- Multiple unassigned literals
+ -- | err                          -- Something went wrong? Helps make proofs easier
+
+  -- Note: ResultT is the Exception monad, renamed.
+  open ResultT
+  open PropagateResult PropagateResultDep
+
+  abbrev Box := ResultT PPR (Option ILit)
+
+  def propUnitFun (τ : PPA) (box : Option ILit) (lit : ILit) : Box :=
+    match τ.litValue? lit with
+    | some true  => done .satisfied
+    | some false => ok box
+    | none =>
+        match box with
+        | none => ok lit
+        | some u =>
+          if u != lit then
+            done .multipleUnassignedLiterals
+          else
+            ok box
+
+  def propagate (τ : PPA) (C : IClause) := C.foldlM (propUnitFun τ) none
+
+  def propagateUnit (τ : PPA) (C : IClause) : PropagateResult :=
+    match propagate τ C with
+    | ok none => .contradiction
+    | ok (some lit) => .extended lit (τ.setLit lit)
+    | done .satisfied => .satisfied
+    | done .multipleUnassignedLiterals => .multipleUnassignedLiterals
+
+  theorem pu_sm2 (τ : PPA) (C : IClause) :
+      SatisfiesM (fun
+        | none => ∀ l ∈ C.data, τ.litValue? l = some false
+        | some lit => lit ∈ C.data ∧ τ.litValue? lit = none ∧
+          ∀ l ∈ C.data, l ≠ lit → τ.litValue? l = some false) (propagate τ C) := by
+    -- Cayden TODO: Why do I have to supply the hypothesis here? And not C[i]?
+    have := C.SatisfiesM_foldlM (init := none) (f := propUnitFun τ)
+      (motive := fun
+        | idx, none => ∀ ⦃i : Fin C.size⦄, i < idx → τ.litValue? (C[i.val]'i.isLt) = some false
+        | idx, some lit => lit ∈ C.data ∧ τ.litValue? lit = none ∧
+          ∀ ⦃j : Fin C.size⦄, j < idx → C[j.val]'j.isLt ≠ lit → τ.litValue? (C[j]'j.isLt) = some false)
+      (h0 := by simp)
+      (hf := by
+        simp only [SatisfiesM_ResultT_eq, getElem_fin]
+        intro i box ih
+        -- Cayden question: Is this proof more compact if I use pattern-matching with intro?
+        intro
+        | none, hbox =>
+          simp only
+          intro j hj
+          unfold propUnitFun at hbox
+          cases h_tau : τ.litValue? C[i.val] with
+          | none =>
+            simp [h_tau] at hbox
+            cases h_box : box with
+            | none => simp [h_box] at hbox
+            | some lit => by_cases h_lit : lit = C[i.val] <;> simp [h_box, h_lit] at hbox
+          | some b =>
+            cases h_box : box with
+            | none =>
+              subst h_box
+              rcases lt_or_eq_of_le (le_of_lt_succ hj) with (h | h)
+              · exact ih h
+              · cases b
+                · replace h := Fin.ext h; subst h; exact h_tau
+                · simp [h_tau] at hbox
+            | some lit => by_cases h_lit : lit = C[i.val] <;> cases b <;> simp [h_tau, h_box, h_lit] at hbox
+        | some lit, hbox =>
+          unfold propUnitFun at hbox
+          cases h_tau : τ.litValue? C[i.val] with
+          | none =>
+            simp [h_tau] at hbox
+            cases h_box : box with
+            | none =>
+              subst h_box
+              simp at hbox
+              use Array.mem_data_iff.mpr ⟨i, hbox⟩, hbox ▸ h_tau
+              intro j hj₁ hj₂
+              rcases lt_or_eq_of_le (le_of_lt_succ hj₁) with (h | h)
+              · exact ih h
+              · simp at ih
+                replace h := Fin.ext h; subst h; rw [hbox] at hj₂; contradiction
+            | some l =>
+              subst h_box
+              by_cases hl : l = C[i.val]
+              · simp [hl] at hbox
+                rw [hbox] at hl
+                subst hl
+                rcases ih with ⟨hl₁, hl₂, ih⟩
+                use hl₁, hl₂
+                intro j hj₁ hj₂
+                rcases lt_or_eq_of_le (le_of_lt_succ hj₁) with (h | h)
+                · exact ih h hj₂
+                · replace h := Fin.ext h; subst h; rw [hbox] at hj₂; contradiction
+              · simp [hl] at hbox
+          | some b =>
+            cases b
+            · simp [h_tau] at hbox
+              subst hbox
+              rcases ih with ⟨hlit₁, hlit₂, ih⟩
+              use hlit₁, hlit₂
+              intro j hj₁ hj₂
+              rcases lt_or_eq_of_le (le_of_lt_succ hj₁) with (h | h)
+              · exact ih h hj₂
+              · replace h := Fin.ext h; subst h; exact h_tau
+            · simp [h_tau] at hbox)
+    apply SatisfiesM.imp this
+    intro
+    | none =>
+      intro h l hl
+      rcases Array.mem_data_iff.mp hl with ⟨i, rfl⟩
+      exact h i.isLt
+    | some lit =>
+      simp
+      intro hlit₁ hlit₂ ih
+      use hlit₁, hlit₂
+      intro l hl₁ hl₂
+      rcases Array.mem_data_iff.mp hl₁ with ⟨i, rfl⟩
+      exact ih hl₂
+
+  theorem propUnit_contradiction {τ : PPA} {C : IClause} :
+      propagateUnit τ C = .contradiction → C.toPropFun ⊓ τ.toPropFun ≤ ⊥ := by
+    intro hpu
+    unfold propagateUnit at hpu
+    cases hp : propagate τ C with
+    | ok box =>
+      cases box with
+      | none =>
+        clear hpu
+        refine entails_ext.mpr fun σ hσ => ?_
+        rw [satisfies_conj] at hσ
+        rcases hσ with ⟨hσ₁, hσ₂⟩
+        have ⟨lit, hlit, hσlit⟩ := Clause.satisfies_iff.mp hσ₁
+        have hvar := satisfies_iff'.mp hσ₂ lit false (SatisfiesM_ResultT_eq.mp (pu_sm2 τ C) none hp lit hlit)
+        simp [LitVar.satisfies_iff.mp hσlit] at hvar
+        cases hpol : polarity lit <;> rw [hpol] at hvar <;> contradiction
+      | some lit => simp [hp] at hpu
+    | done ppr => cases ppr <;> simp [hp] at hpu
+
+  theorem propUnit_extended {τ τ' : PPA} {C : IClause} {l : ILit} :
+      propagateUnit τ C = .extended l τ' →
+        C.toPropFun ⊓ τ.toPropFun ≤ τ'.toPropFun ∧
+        τ.litValue? l = none ∧
+        τ'.litValue? l = some true := by
+    intro hpu
+    unfold propagateUnit at hpu
+    cases hp : propagate τ C with
+    | ok box =>
+      cases box with
+      | none => simp [hp] at hpu
+      | some lit =>
+        simp [hp] at hpu
+        rcases hpu with ⟨rfl, rfl⟩
+        have ⟨hl₁, hl₂, hl₃⟩ := SatisfiesM_ResultT_eq.mp (pu_sm2 τ C) _ hp
+        constructor
+        · refine entails_ext.mpr fun σ hσ => ?_
+          rw [satisfies_conj] at hσ
+          rcases hσ with ⟨hσ₁, hσ₂⟩
+          rw [satisfies_iff] at hσ₂
+          -- Cayden TODO: rename these hypotheses
+          rcases Clause.satisfies_iff.mp hσ₁ with ⟨m, hm₁, hm₂⟩
+          rw [LitVar.satisfies_iff] at hm₂
+          rw [satisfies_iff]
+          intro v b hv
+          by_cases hvl : v = (toVar lit)
+          · rw [setLit_varValue_pos τ hvl] at hv
+            injection hv with hv
+            by_cases hlm : m = lit
+            · subst hlm
+              rw [← hvl, hv] at hm₂
+              exact hm₂
+            · have := litValue?_eq_varValue?_some (hl₃ m hm₁ hlm)
+              simp [← hm₂] at this
+              replace this := hσ₂ _ _ this
+              -- Cayden question: Why can't `contradiction` work here?
+              cases hs : σ (toVar m) <;> rw [hs] at this <;> contradiction
+          · rw [setLit_varValue_neg τ (Ne.symm hvl)] at hv
+            exact hσ₂ _ _ hv
+        · use hl₂, setLit_pos _ _
+    | done ppr => cases ppr <;> simp [hp] at hpu
+
+  theorem propUnit_satisfied {τ : PPA} {C : IClause} :
+      propagateUnit τ C = .satisfied →
+        -- Cayden TODO: Better way to express that τ ⊨ C?
+        ⊤ ≤ C.toPropFun ⊓ τ.toPropFun := by
+    intro hpu
+    refine entails_ext.mpr fun σ hσ => ?_
+    clear hσ
+    rw [satisfies_conj]
+    --have := SatisfiesM_ResultT_
+    constructor
+    · sorry
+      done
+    sorry
+    done
+
+  def motive (τ : PPA) (C : IClause) : Nat → Option ILit → Prop := fun idx box =>
+    (hidx : idx ≤ C.size) → box = none → ∀ ⦃i : Nat⦄, (hi : i < idx) → τ.litValue? (C.get ⟨i, lt_of_lt_of_le hi hidx⟩) = some false
+
+  theorem propUnit_fold_satisfied {τ : PPA} {C : IClause} :
+      C.foldlM (propUnitFun τ) none = ok none → ∀ (i : Fin C.size), τ.litValue? C[i] = false := by
+    have : SatisfiesM (motive τ C C.size) (C.foldlM (propUnitFun τ) none) := by
+      apply Array.SatisfiesM_foldlM
+      · intro hidx _ i hi; contradiction
+      · intro i box hmotive
+        unfold propUnitFun
+        cases h_tau : τ.litValue? C[i] with
+        | none =>
+          cases h_box : box with
+          | none =>
+            simp
+            have : motive τ C (↑i + 1) (some C[↑i]) := by intro _ h; contradiction
+            exact this
+          | some lit =>
+            by_cases hlit : lit = C[↑i]
+            · simp [hlit]
+              have : motive τ C (↑i + 1) (some C[↑i]) := by intro _ h; contradiction
+              exact this
+            · rw [getElem_fin] at hlit
+              simp [hlit]
+        | some b =>
+          cases b
+          · simp [h_tau]
+            have : motive τ C (↑i + 1) box := by
+              rintro hidx rfl j hj
+              rcases Nat.eq_or_lt_of_le (Nat.le_of_lt_succ hj) with (rfl | h)
+              · simp; exact h_tau
+              · exact hmotive Fin.is_le' rfl h
+            exact this
+          · simp [h_tau]
+    intro h_fold i
+    unfold SatisfiesM at this
+    rcases this with ⟨x, hx⟩
+    rw [h_fold] at hx
+    cases hx_type : x with
+    | ok y =>
+      subst hx_type
+      rcases y with ⟨y, hy⟩
+      cases y with
+      | none => exact hy (le_refl _) rfl i.isLt
+      | some l =>
+        simp only [Applicative.toFunctor, Monad.toApplicative, instMonadResultT,
+          ResultT.bind, Function.comp_apply, ok.injEq] at hx
+    | done y =>
+      subst hx_type
+      contradiction
+
+  #exit
+
+  /-
+  inductive UnitPropResultDep {α : Type} [BEq α] [Hashable α]
+    (db : ClauseDb α) (σ : PartPropAssignment) (hints : Array α) where
+  /-- A contradiction was derived. The contradiction is implied by the subset of the database
+  used in hints as well as the initial assignment. -/
+  | contradiction (h : db.toPropTermSub (· ∈ hints.data) ⊓ σ.toPropTerm ≤ ⊥)
+  /-- The partial assignment was extended. The final assignment `σ'` is implied by the subset of
+  the database used in hints as well as the initial assignment. -/
+  | extended (σ' : PartPropAssignment)
+             (h : db.toPropTermSub (· ∈ hints.data) ⊓ σ.toPropTerm ≤ σ'.toPropTerm)
+  /-- The hint `C` at index `idx` did not become unit under `σ`. -/
+  | hintNotUnit (idx : α) (C : IClause) (σ : PartPropAssignment)
+  /-- The hint index `idx` points at a nonexistent clause. -/
+ | hintNonexistent (idx : α)
+  -/
+
+  /-- If `C` is satisfied by `τ`, return `notUnit`.
+  Otherwise compute the reduced clause `C' = {l ∈ C | ¬l ∉ τ}`.
+  If `C' = [u]` is a unit, extend `τ` by `u` and return `extended`.
+  If `C'` has become empty (is falsified), return `contradiction`.
+  If `C'` is not a unit and not falsified, return `notUnit`. -/
+  def propagateUnit (τ : PPA) (C : IClause) :
+      PropagateResultDep τ C := Id.run do
+    -- The candidate for a unit.
+    -- The ILit is the value stored in the clause, while the Fin is the index in the clause to access it
+    --let mut unit? : Option ((i : ILit) × { f : Fin C.size // C[f] = i }) := none
+    --let mut unit? : Option ILit := none
+    let mut unitIdx? : Option ({i : Fin C.size // τ.litValue? C[i] = none}) := none
+    let mut idx : { idx : Fin (C.size + 1) //
+      (unitIdx? = none → ∀ (i : Fin idx), τ.litValue? C[i] = some false) ∧
+      (unitIdx? ≠ none → ∃ v : ({i : Fin C.size // τ.litValue? C[i] = none}),
+        unitIdx? = some v ∧
+        ∀ (i : Fin idx), i.val ≠ v.val.val → τ.litValue? C[i] = some false ) } :=
+          ⟨0, sorry⟩
+
+    for hi : i in [0:C.size] do
+      have hi_lt : i < C.size := Membership.mem.upper hi
+      let l := C[i]'hi_lt
+      have hl : l ∈ C.data := Array.getElem_mem_data C _
+      match hl_val : τ.litValue? l with
+      | some true => return .notUnit
+      | some false =>
+          -- Maintain invariant
+
+          continue
+      | none =>
+          match unitIdx? with
+          | none => unitIdx? := ⟨some l, fun _ => ⟨l, hl, sorry⟩⟩
+          | some ⟨j, h⟩ =>
+            if i ≠ j.val then return .notUnit
+      continue
+          --if let .some ⟨j, h⟩ := unitIdx? then
+          --  if i ≠ j.val then
+          --    return .notUnit
+
+      -- Update invariant
+
+
+
+    if hIdx : idx.val = C.size then
+      match unitIdx? with
+      | none => return .contradiction
+      | some ⟨i, h⟩ => return .extended C[i] (τ.setLit C[i])
+    else
+      return .err
+
+#check List.foldl
+
+#exit
+
+/-
+def unitPropWithHintsDep (db : ClauseDb α) (σ₀ : PartPropAssignment) (hints : Array α)
+    : UnitPropResultDep db σ₀ hints := Id.run do
+  let mut σ : {σ : PartPropAssignment //
+      db.toPropTermSub (· ∈ hints.data) ⊓ σ₀.toPropTerm ≤ σ.toPropTerm } :=
+    ⟨σ₀, inf_le_right⟩
+  for h : i in [0:hints.size] do
+    let hint := hints[i]'(Membership.mem.upper h)
+    have hMem : hint ∈ hints.data := Array.getElem_mem_data hints _
+
+    match hGet : db.getClause hint with
+    | none => return .hintNonexistent hint
+    | some C =>
+      have hDbσ₀ :
+          db.toPropTermSub (· ∈ hints.data) ⊓ σ₀.toPropTerm ≤ C.toPropTerm ⊓ σ.val.toPropTerm :=
+        le_inf (inf_le_of_left_le (toPropTermSub_of_getClause_eq_some db hMem hGet)) σ.property
+      match hRed : C.reduce σ.val with
+      | some #[] =>
+        have : db.toPropTermSub (· ∈ hints.data) ⊓ σ₀.toPropTerm ≤ ⊥ := by
+          have : C.toPropTerm ⊓ σ.val.toPropTerm ≤ ⊥ :=
+            IClause.reduce_eq_some _ _ _ hRed
+          exact le_trans hDbσ₀ this
+        return .contradiction this
+      | some C' =>
+        let some ⟨u, hU⟩ := checkIsUnit C'
+          | return .hintNotUnit hint C σ.val
+        have : db.toPropTermSub (· ∈ hints.data) ⊓ σ₀.toPropTerm ≤
+            PartPropAssignment.toPropTerm (σ.val.insert u.var u.polarity) := by
+          have hU : db.toPropTermSub (· ∈ hints.data) ⊓ σ₀.toPropTerm ≤ u.toPropTerm := by
+            have h := IClause.reduce_eq_some _ _ _ hRed
+            conv at h => rhs; rw [← hU]; simp [IClause.toPropTerm]
+            exact le_trans hDbσ₀ h
+          refine PropTerm.entails_ext.mpr fun τ hτ => ?_
+          have hU : τ ⊨ u.toPropTerm :=
+            PropTerm.entails_ext.mp hU τ hτ
+          have hσ : τ ⊨ σ.val.toPropTerm :=
+            PropTerm.entails_ext.mp σ.property τ hτ
+          rw [PartPropAssignment.satisfies_iff] at hσ ⊢
+          intro x p hFind
+          by_cases hEq : x = u.var
+          next =>
+            rw [hEq, HashMap.find?_insert _ _ LawfulBEq.rfl] at hFind
+            rw [ILit.satisfies_iff] at hU
+            simp_all
+          next =>
+            rw [HashMap.find?_insert_of_ne _ _ (bne_iff_ne _ _ |>.mpr (Ne.symm hEq))] at hFind
+            exact hσ _ _ hFind
+        σ := ⟨σ.val.insert u.var u.polarity, this⟩
+      | _ => return .hintNotUnit hint C σ.val
+  return .extended σ.val σ.property
+-/
+
+end PPA
